rearranged_code/inverse.v
@@ -1,8 +1,27 @@
 Require Import Omega.
+Require Import Program.Basics.
 Require Import Logic.FunctionalExtensionality.
 Require Import prelims.
 Require Import repeater.
 Require Import increasing_expanding.
+
+(*
+===================================================================================
+**** SECTION 3.1 INCREASING FUNCTIONS, UPPER INVERSE AND EXPANSIONS (2)************
+===================================================================================
+ *)
+
+(* In Section 3.1, we introduce the notion of "upper inverse" (upp_inv),
+   increasing functions and why we prefer to consider inverse of
+   increasing functions only.
+   We prove several use results about upper inverse and increasing functions
+   We introduce "expansions" and how they are connected to increasing functions
+   through repeater.
+   Increasing functions that are strict expansions serve as the target for us
+   to compute the upper inverse with "countdown" later on. *)
+
+(* In this PART 2 file, we deal with upper inverse of increasing functions *)
+
 
 (* ****** UPPER INVERSE ****************** *)
 
@@ -12,7 +31,12 @@ Definition upp_inv_rel (f F : nat -> nat) : Prop :=
 
 (* An increasing F has a recursively definable upper inverse
    Under assumption F is increasing, the below definition will compute its upper inverse
-   Do not use it for not always increasing functions *)
+   Do not use it for not always increasing functions
+   This is sort of why we are only interested in inverses of increasing functions
+   Inverses of other functions on naturals are hard to define neatly and do not
+   behave nicely.
+   This computation implies the upper inverse exists, which is useful for
+   proofs about worker functions later on *)
 Fixpoint upp_inv (F : nat -> nat) (n : nat) : nat :=
   match n with
   | 0 => 0
@@ -55,6 +79,20 @@ Proof.
   - rewrite H0. trivial.
 Qed.
 
+(* Composing F's inverse and F gives identity *)
+Theorem upp_inv_compose :
+    forall f F, increasing F -> upp_inv_rel f F -> compose f F = id.
+Proof.
+  intros f F HF HfF. apply functional_extensionality. intro n.
+  unfold id. unfold compose.
+  assert (f (F n) <= n) as H0.
+  { rewrite (HfF n (F n)). trivial. }
+  assert (n <= f (F n)) as H1.
+  { rewrite not_lt. rewrite (incr_twoways F (f (F n)) n HF).
+    rewrite <- not_lt. rewrite <- (HfF (f (F n)) (F n)). trivial. }
+  omega.
+Qed.
+
 (* Repeat preserves upper inverse relation *)
 Lemma upp_inv_repeat : forall k f F,
     upp_inv_rel f F -> upp_inv_rel (repeat f k) (repeat F k).
@@ -65,87 +103,3 @@ Proof.
   - intro. rewrite IHk in H. simpl. apply HfF. apply H.
   - simpl; rewrite <- HfF; rewrite IHk; trivial.
 Qed.
-
-(* The inverse of (repeater_from a F) is the minimum number of applications
-   of (inverse F) to the input to get a result less than or equal to a.
-   This serves as motivation to countdown (later on) and contractions. *)
-Lemma upp_inv_repeater : forall a f F f',
-    upp_inv_rel f F -> upp_inv_rel f' (repeater_from F a)
-    -> (forall n m, f' n <= m <-> repeat f m n <= a).
-Proof.
-  intros a f F f' HfF Hf'F n m.
-  rewrite (Hf'F m n). rewrite repeater_from_repeat.
-  symmetry. apply (upp_inv_repeat m f F HfF a n).
-Qed.
-
-(* ****** CONTRACTIONS ****************** *)
-
-(* Definition of non-strict contractions *)
-Definition contracting (f : nat -> nat) : Prop :=
-  forall n, f n <= n.
-
-(* Definition of strict expansion *)
-Definition contract_strict_above (a : nat) (f : nat -> nat) : Prop :=
-  contracting f /\ (forall n, S a <= n -> S (f n) <= n).
-
-(* Upper inverse of expansions are contractions *)
-Theorem upp_inv_expand_contract :
-    forall f F, expanding F -> upp_inv_rel f F -> contracting f.
-Proof.
-  intros f F HF HfF n. rewrite (HfF n n). apply HF.
-Qed.
-
-(* Upper inverse of strict from a expansions contract above a *)
-Theorem upp_inv_expand_contract_strict :
-    forall a f F, expand_strict_from a F -> upp_inv_rel f F -> contract_strict_above a f.
-Proof.
-  intros a f F HF HfF. destruct HF as [HF HaF].
-  split.
-  - apply (upp_inv_expand_contract _ F); assumption.
-  - intro n. destruct n; [omega|]. repeat rewrite <- le_S_n_m.
-    rewrite (HfF n _). apply HaF.
-Qed.
-
-(* ****** PROPERTIES OF CONTRACTIONS ************ *)
-
-(* repeat of contractions make the result smaller *)
-Lemma repeat_contract :
-  forall f n k l,
-    contracting f -> k <= l -> repeat f l n <= repeat f k n.
-Proof.
-  intros f n k l Hf Hkl. induction l; inversion Hkl; trivial.
-  apply IHl in H0.
-  apply (Nat.le_trans _ (repeat f l n) _); [apply Hf | apply H0].
-Qed.
-
-(* strict version *)
-Lemma repeat_contract_strict :
-  forall a f n k,
-    contract_strict_above a f ->
-    S a <= repeat f k n -> (S k) + repeat f (S k) n <= n.
-Proof.
-  intros a f n k Hf Han. destruct Hf as [Hf Haf]. induction k.
-  1: simpl in Han; simpl; apply Haf in Han; omega. 
-  apply (Nat.le_trans _ (S k + repeat f (S k) n) _).
-  - apply Haf in Han. simpl. simpl in Han. omega.
-  - assert (S a <= repeat f k n) as Han0.
-    { apply (Nat.le_trans _ (repeat f (S k) n) _); [apply Han|].
-      apply Haf in Han. simpl. apply Hf. }
-    apply IHk in Han0. omega.
-Qed.
-
-
-(* 
- * Cleaning up to replace "S a <= b" with "a < b".
- * The exact same proof works. 
- *)
-Lemma repeat_contract_strict' :
-  forall a f n k,
-    contract_strict_above a f ->
-    a < repeat f k n ->
-    k + repeat f (S k) n < n.
-Proof. apply repeat_contract_strict. Qed.
-(* 
- * I wonder if maybe we can replace it like this everywhere,
- * provided it doens't affect the computation.
- *)
